\section{Stevens Operators}\label{stevens}

\begin{eqnarray*}
X=J(J+1)\\
O_{00}&=&1\\
\hline
O^s_{11}&=&\frac{-i}{2}[J_+-J_-]=J_y \\
O_{10}&=&J_z \\
O_{11}&=&\frac{1}{2}[J_++J_-]=J_x \\
\hline
O^s_{22}&=&\frac{-i}{2}[J_+^2-J_-^2]=J_xJ_y+J_yJ_x=2P_{xy} \\
O^s_{21}&=&\frac{-i}{4}[J_z(J_+-J_-)+(J_+-J_-)J_z]=\frac{1}{2}[J_yJ_z+J_zJ_y]=P_{yz} \\
O_{20}&=&[3J_z^2-X] \\
O_{21}&=&\frac{1}{4}[J_z(J_++J_-)+(J_++J_-)J_z]=\frac{1}{2}[J_xJ_z+J_zJ_x]=P_{xz} \\
O_{22}&=&\frac{1}{2}[J_+^2+J_-^2]=J_x^2-J_y^2 \\
\hline
O^s_{33}&=&\frac{-i}{2}[J_+^3-J_-^3] \\
O^s_{32}&=&\frac{-i}{4}[(J_+^2-J_-^2)J_z+J_z(J_+^2-J_-^2)] \\
O^s_{31}&=&\frac{-i}{4}[(J_+-J_-)(5J_z^2-X-1/2)+(5J_z^2-X-1/2)(J_+-J_-)] \\
O_{30}&=&[5J_z^3-(3X-1)J_z] \\
O_{31}&=&\frac{1}{4}[(J_++J_-)(5J_z^2-X-1/2)+(5J_z^2-X-1/2)(J_++J_-)] \\
O_{32}&=&\frac{1}{4}[(J_+^2+J_-^2)J_z+J_z(J_+^2+J_-^2)] \\
O_{33}&=&\frac{1}{2}[J_+^3+J_-^3] \\
\hline
O^s_{44}&=&\frac{-i}{2}[(J_+^4-J_-^4]\\
O^s_{43}&=&\frac{-i}{4}[(J_+^3-J_-^3)J_z+J_z(J_+^3-J_-^3)] \\
O^s_{42}&=&\frac{-i}{4}[(J_+^2-J_-^2)(7J_z^2-X-5)+(7J_z^2-X-5)(J_+^2-J_-^2)] \\
O^s_{41}&=&\frac{-i}{4}[(J_+-J_-)(7J_z^3-(3X+1)J_z)+(7J_z^3-(3X+1)J_z)(J_+-J_-)] \\
O_{40}&=&[35J_z^4-(30X-25)J_z^2+3X^2-6X] \\
O_{41}&=&\frac{1}{4}[(J_++J_-)(7J_z^3-(3X+1)J_z)+(7J_z^3-(3X+1)J_z)(J_++J_-)] \\
O_{42}&=&\frac{1}{4}[(J_+^2+J_-^2)(7J_z^2-X-5)+(7J_z^2-X-5)(J_+^2+J_-^2)] \\
O_{43}&=&\frac{1}{4}[(J_+^3+J_-^3)J_z+J_z(J_+^3+J_-^3)] \\
O_{44}&=&\frac{1}{2}[(J_+^4+J_-^4]\\
\hline
O^s_{55}&=&\frac{-i}{2}[J_+^5-J_-^5] \\
O^s_{54}&=&\frac{-i}{4}[(J_+^4-J_-^4)J_z+J_z(J_+^4-J_-^4)] \\
O^s_{53}&=&\frac{-i}{4}[(J_+^3-J_-^3)(9J_z^2-X-33/2)+(9J_z^2-X-33/2)(J_+^3-J_-^3)] \\
O^s_{52}&=&\frac{-i}{4}[(J_+^2-J_-^2)(3J_z^3-(X+6)J_z)+(3J_z^3-(X+6)J_z)(J_+^2-J_-^2)]\\
O^s_{51}&=&\frac{-i}{4}[(J_+-J_-)\{21J_z^4-14J_z^2X+X^2-X+3/2\}+\{\dots\}(J_+-J_-)] \\
O_{50}&=&[63J_z^5-(70X-105)J_z^3+(15X^2-50X+12)J_z] \\
O_{51}&=&\frac{1}{4}[(J_++J_-)(21J_z^4-14J_z^2X+X^2-X+3/2)+(21J_z^4-14J_z^2X+X^2-X+3/2)(J_++J_-)] \\
O_{52}&=&\frac{1}{4}[(J_+^2+J_-^2)(3J_z^3-(X+6)J_z)+(3J_z^3-(X+6)J_z)(J_+^2+J_-^2)] \\
O_{53}&=&\frac{1}{4}[(J_+^3+J_-^3)(9J_z^2-X-33/2)+(9J_z^2-X-33/2)(J_+^3+J_-^3)] \\
O_{54}&=&\frac{1}{4}[(J_+^4+J_-^4)J_z+J_z(J_+^4+J_-^4)] \\
O_{55}&=&\frac{1}{2}[J_+^5+J_-^5] \\
\hline
O^s_{66}&=&\frac{-i}{2}[J_+^6-J_-^6]\\
O^s_{65}&=&\frac{-i}{4}[(J_+^5-J_-^5)J_z+J_z(J_+^5-J_-^5)] \\
O^s_{64}&=&\frac{-i}{4}[(J_+^4-J_-^4)(11J_z^2-X-38)+(11J_z^2-X-38)(J_+^4-J_-^4)] \\
O^s_{63}&=&\frac{-i}{4}[(J_+^3-J_-^3)(11J_z^3-(3X+59)J_z)+(11J_z^3-(3X+59)J_z)(J_+^3-J_-^3)] \\
O^s_{62}&=&\frac{-i}{4}[(J_+^2-J_-^2)\{33J_z^4-(18X+123)J_z^2+X^2+10X+102\}+\{\dots\}(J_+^2-J_-^2)] \\
O^s_{61}&=&\frac{-i}{4}[(J_+-J_-)\{33J_z^5-(30X-15)J_z^3+(5X^2-10X+12)J_z\}+\{\dots\}(J_+-J_-)] \\
O_{60}&=&[231J_z^6-(315X-735)J_z^4+(105X^2-525X+294)J_z^2-5X^3+40X^2-60X] \\
O_{61}&=&\frac{1}{4}[(J_++J_-)\{33J_z^5-(30X-15)J_z^3+(5X^2-10X+12)J_z\}+\{\dots\}(J_++J_-)] \\
O_{62}&=&\frac{1}{4}[(J_+^2+J_-^2)\{33J_z^4-(18X+123)J_z^2+X^2+10X+102\}+\{\dots\}(J_+^2+J_-^2)] \\
O_{63}&=&\frac{1}{4}[(J_+^3+J_-^3)(11J_z^3-(3X+59)J_z)+(11J_z^3-(3X+59)J_z)(J_+^3+J_-^3)] \\
O_{64}&=&\frac{1}{4}[(J_+^4+J_-^4)(11J_z^2-X-38)+(11J_z^2-X-38)(J_+^4+J_-^4)] \\
O_{65}&=&\frac{1}{4}[(J_+^5+J_-^5)J_z+J_z(J_+^5+J_-^5)] \\
O_{66}&=&\frac{1}{2}[J_+^6+J_-^6]\\
\end{eqnarray*}



